QsADTs: Tuples0F insertion

Bedrock/Platform/Facade/examples/Tuples0F.v
@@ -9,9 +9,10 @@ Section tuples0.
   Open Scope Sep_scope.
 
   Definition tuples0 (len : nat) (ts : tuples) (p : W) :=
-    Ex ls, Ex lsp, (p ==*> natToW len, lsp) * lseq ls lsp * [| EnsembleIndexedListEquivalence ts ls |]
+    Ex ls, Ex lsp, Ex bound, (p ==*> natToW len, lsp) * lseq ls lsp * [| EnsembleIndexedListEquivalence ts ls |]
       * [| $2 <= natToW len |]
-      * [| forall t, IndexedEnsemble_In ts t -> length t = len |].
+      * [| forall t, IndexedEnsemble_In ts t -> length t = len |]
+      * [| UnConstrFreshIdx ts bound |].
 End tuples0.
 
 Definition Empty : tuples := fun _ => False.
@@ -20,8 +21,13 @@ Definition newS := SPEC("extra_stack", "len") reserving 11
   PRE[V] [| V "len" >= $2 |] * mallocHeap 0
   POST[R] tuples0 (wordToNat (V "len")) Empty R * mallocHeap 0.
 
+Definition pushS := SPEC("extra_stack", "self", "tup") reserving 12
+  Al len, Al ts, Al t,
+  PRE[V] tuples0 len ts (V "self") * tuple t (V "tup") * [| length t = len |] * mallocHeap 0
+  POST[R] [| R = $0 |] * Ex ts', [| insert ts t ts' |] * tuples0 len ts' (V "self") * mallocHeap 0.
+
 Definition m := bimport [[ "malloc"!"malloc" @ [mallocS], "malloc"!"free" @ [freeS],
-                           "TupleList"!"new" @ [TupleListF.newS] ]]
+                           "TupleList"!"new" @ [TupleListF.newS], "TupleList"!"push" @ [TupleListF.pushS] ]]
   bmodule "Tuples0" {{
     bfunction "new"("extra_stack", "len", "x") [newS]
       "x" <-- Call "malloc"!"malloc"(0, 2)
@@ -36,6 +42,15 @@ Definition m := bimport [[ "malloc"!"malloc" @ [mallocS], "malloc"!"free" @ [fre
       "x" *<- "len";;
       "x" + 4 *<- "extra_stack";;
       Return "x"
+    end
+
+    with bfunction "push"("extra_stack", "self", "tup") [pushS]
+      "self" <-* "self" + 4;;
+      "self" <-- Call "TupleList"!"push"("extra_stack", "self", "tup")
+      [PRE[_] Emp
+       POST[R] [| R = $0 |] ];;
+
+      Return 0
     end
   }}.
 
@@ -68,15 +83,87 @@ Hint Extern 1 (_ = wordToNat _) =>
   | [ H : IndexedEnsemble_In Empty _ |- _] => destruct H as [ ? [ ] ]
   end.
 
+Lemma fresh_Empty : UnConstrFreshIdx Empty O.
+Proof.
+  hnf; destruct 1.
+Qed.
+
+Hint Resolve fresh_Empty.
+
+Definition insertAt (ts : tuples) (idx : nat) (t : tupl) : tuples :=
+  EnsembleInsert {| elementIndex := idx;
+                    indexedElement:= t |} ts.
+
+Theorem insert_insertAt : forall ts idx t,
+  UnConstrFreshIdx ts idx
+  -> insert ts t (insertAt ts idx t).
+Proof.
+  unfold insert, insertAt, UnConstrFreshIdx, Ensembles.In; simpl; intros.
+  exists idx; intuition subst.
+  apply H in H0; omega.
+Qed.
+
+Hint Immediate insert_insertAt.
+
+Theorem EnsembleIndexedListEquivalence_insertAt : forall ts idx t ls,
+  UnConstrFreshIdx ts idx
+  -> EnsembleIndexedListEquivalence ts ls
+  -> EnsembleIndexedListEquivalence (insertAt ts idx t) (t :: ls).
+Proof.
+  unfold insertAt, EnsembleIndexedListEquivalence, UnIndexedEnsembleListEquivalence, UnConstrFreshIdx, EnsembleInsert, Ensembles.In; simpl; firstorder idtac.
+  exists (S idx); intuition subst; simpl; intuition.
+  exists ({| elementIndex := idx; indexedElement := t |} :: x0); simpl; intuition.
+  firstorder idtac.
+  firstorder idtac.
+  constructor; auto.
+  intro.
+  apply in_map_iff in H4; destruct H4; intuition subst.
+  apply H2 in H6.
+  apply H in H6.
+  omega.
+Qed.
+
+Hint Immediate EnsembleIndexedListEquivalence_insertAt.
+
+Theorem bounded_insertAt : forall ts idx t t',
+  (forall t'', IndexedEnsemble_In ts t'' -> length t'' = length t)
+  -> IndexedEnsemble_In (insertAt ts idx t) t'
+  -> length t' = length t.
+Proof.
+  unfold insertAt, IndexedEnsemble_In, EnsembleInsert, Ensembles.In; simpl; firstorder congruence.
+Qed.
+
+Hint Immediate bounded_insertAt.
+
+Theorem fresh_insertAt : forall ts idx t,
+  UnConstrFreshIdx ts idx
+  -> UnConstrFreshIdx (insertAt ts idx t) (S idx).
+Proof.
+  unfold insertAt, UnConstrFreshIdx, EnsembleInsert, Ensembles.In; simpl; firstorder idtac.
+  subst; simpl; omega.
+  firstorder omega.
+Qed.
+
+Hint Immediate fresh_insertAt.
+
 Theorem ok : moduleOk m.
 Proof.
   vcgen.
 
-  Ltac t := unfold tuples0; sep_auto; eauto.
+  Ltac t := solve [ unfold tuples0; sep_auto; eauto ].
 
   t.
   t.
   t.
+  t.
+  t.
+  t.
+  t.
+  t.
+  t.
+  t.
+  t.
+
   t.
   t.
   t.
